# Exercise 2.1
i) $S^{2}\le \frac{1}{n-1}\sum\limits_{i}^n{(X_{i}-a)^2}$ for any $a\in\mathbb{R}$ 
$S^{2} =\frac{1}{n-1}\sum\limits_{i}^n{(X_{i}-\overline X)^2}\le \frac{1}{n-1}\sum\limits_{i}^n{(X_{i}-a)^2}$
$\sum\limits_{i}^n{(X_{i}-\overline X)^2}\le \sum\limits_{i}^n{(X_{i}-a)^2}$
$\sum\limits_{i}^n{(-2X_{i}\overline X +\overline{X}^2)}\le \sum\limits_{i}^n{(-2X_{i}a +{a}^2)}$
$\sum\limits_{i}^n{(-2X_{i}\overline X )+n\overline{X}^{2}\le -2a\sum\limits_{i}^{n}}{(X_{i}) +{\sum\limits_{i}^{n}(a^2})}$
$-2 n\overline X^{2}+{n\overline X^{2}\le}-2a n \overline X+ {n a^2}$
$-n\overline X^{2} \le -2a n \overline X+ {n a^2}$
$-\overline X^{2} \le -2a \overline X+ {n^2 a^2}$
$0 \le\overline X^{2} -2a \overline X+ {n^{2} a^{2}}(\star)$
if $a$ and $\overline X$ have the opposite sign the inequality $(\star)$ is true because a sum of positive numbers is $\ge 0$.
otherwise:
$\overline X^{2} -2a \overline X+ {n^{2} a^{2}}\ge^{(n\ge1)}\overline X^{2} -2an \overline X+ {n^{2} a^{2}}= (\overline X - na)^2\ge0$ $\square$ 

ii) $\frac{(n-1)S^2}{n}=\frac{1}{n}\sum\limits_{i}^n{(X_{i}-\overline X)^2}$
$=\frac{1}{n}\sum\limits_{i}^n{(X_i^2-2X_{i}\overline X +\overline{X}^2)}$
$=\overline{X^{2}}-2\overline{X}^2+\overline{X}^{2}=\overline{X^2}-\overline{X}^2$
$\square$
---
# Exercise 2.2
$X_1,\dots,X_{n}$ iid random sample with $X_{i} \sim F$ with continuous $F$.
$\min:\mathbb R^{n}\to\mathbb R$ 

 
